code/experimental/aes-256-cbc/Hacl.Impl.AES_256_CBC.fst
@@ -63,99 +63,6 @@ let aes256_cbc_encrypt out key iv msg msglen =
   pop_frame ();
   padded_len
 
-(*
-
-let aes256_cbc_encrypt out key iv msg msglen =
-  push_frame();
-  assert (16 <> 0);
-  let fullblocks = (msglen /. size 16) *. size 16 in
-  let final = msglen %. size 16 in
-  let msg1 = sub #MUT #uint8 #msglen msg (size 0) fullblocks in
-  let last = sub #MUT #uint8 #msglen msg fullblocks final in
-  let out1 = sub #MUT #uint8 #(msglen +. size 16) out (size 0) fullblocks in
-  let out2 = sub #MUT #uint8 #(msglen +. size 16) out fullblocks (size 16) in
-  assert(disjoint out1 out2);
-  let scratch = create (xkeylen +. size 48) (u8 0) in
-  let kex = sub scratch (size 0) xkeylen in
-  let tmp = sub scratch xkeylen (size 16) in
-  let otmp = sub scratch (xkeylen +. size 16) (size 16) in
-  let ltmp = sub scratch (xkeylen +. size 32) (size 16) in
-  keyExpansion key kex;
-  cbc_encrypt_blocks out1 kex iv msg1 fullblocks (size 0) tmp;
-  let lastfull = if (fullblocks <>. size 0) then sub out1 (fullblocks -. size 16) (size 16)
-                 else iv in
-  update_sub ltmp (size 0) final (sub last (size 0) final);//blit last 0ul ltmp 0ul final;
-  padPKCS ltmp (size 16 -. final) final;
-  xor_block ltmp ltmp lastfull (size 0);
-  cipher otmp ltmp kex;
-  copy out2 otmp;//blit otmp 0ul out2 0ul 16ul;
-  pop_frame()
-*)
-
-(*
-val cbc_decrypt_blocks:
-  out:buffer uint8 ->
-  kex:xkey ->
-  prev:block ->
-  cip:buffer uint8{length cip == length out} ->
-  len:size_t{v len = length cip /\ v len % 16 = 0} ->
-  curr:size_t{v curr <= v len /\ v curr % 16 = 0} ->
-  tmp:block ->
-  Stack unit
-    (requires (fun h -> live h out /\ live h kex /\ live h prev /\ live h cip /\ live h tmp /\
-      disjoint out kex /\ disjoint out prev /\ disjoint out cip /\ disjoint out tmp /\
-      disjoint tmp kex /\ disjoint tmp prev /\ disjoint tmp cip
-    ))
-    (ensures (fun h0 _ h1 -> modifies2 tmp out h0 h1))
-    (decreases (v len - v curr))
-
-let rec cbc_decrypt_blocks out kex prev cip len curr tmp =
-  if curr = len then ()
-  else (
-    assert(v curr < v len /\ v curr % 16 = 0);
-    let cblock = sub #MUT #uint8 #len cip curr (size 16) in
-    let oblock = sub #MUT #uint8 #len out curr (size 16) in
-    inv_cipher tmp cblock kex;
-    xor_block oblock tmp prev (size 0);
-    cbc_decrypt_blocks out kex cblock cip len (curr +. size 16) tmp
-  )
-
-
-val unpadPKCS:
-  tmp:block ->
-  idx:size_t{v idx <= v blocklen} ->
-  Stack (len:size_t{v len <= v blocklen})
-	 (requires (fun h -> live h tmp))
-	 (ensures (fun h0 _ h1 -> modifies1 tmp h0 h1))
-let rec unpadPKCS tmp idx =
-  let pad = tmp.(blocklen -. size 1) in
-  (* Reading the padding is inherently non constant *)
-  let pad32 = Lib.RawIntTypes.size_from_UInt32
-    (FStar.Int.Cast.uint8_to_uint32
-      (Lib.RawIntTypes.u8_to_UInt8 pad))
-   in
-  if pad32 <=. blocklen then pad32
-  else size 0
-
-val unpadISO:
-  tmp:block ->
-  idx:size_t{v idx < v blocklen} ->
-  Stack (len:size_t{v len < v blocklen})
-	 (requires (fun h -> live h tmp))
-	 (ensures (fun h0 _ h1 -> modifies1 tmp h0 h1))
-let rec unpadISO tmp idx =
-   let t = tmp.(idx) in
-   (* Reading the padding is inherently non constant *)
-   if
-     Lib.RawIntTypes.u8_to_UInt8 t =
-       Lib.RawIntTypes.u8_to_UInt8 (u8 0x80)
-   then idx
-   else if Lib.RawIntTypes.u8_to_UInt8 t <>
-      Lib.RawIntTypes.u8_to_UInt8 (u8 0x00)
-   then 0ul
-   else if idx = 0x0ul then 0ul
-   else unpadISO tmp (idx -. size 1)
-
 val aes256_cbc_decrypt:
   out:buffer uint8 ->
   key:lbuffer uint8 keylen ->
@@ -171,10 +78,12 @@ val aes256_cbc_decrypt:
 
 let aes256_cbc_decrypt out key iv cip ciplen =
   push_frame();
-  let kex = create xkeylen (u8 0) in
-  let tmp = create (size 16) (u8 0) in
-  keyExpansion key kex;
-  cbc_decrypt_blocks out kex iv cip ciplen 0ul tmp;
+   Hacl.Impl.AES_256.Bitsliced.decrypt_blocks_cbc
+    out
+    key
+    iv
+    cip
+    ciplen;
   let pad = index #MUT #uint8 #ciplen out (ciplen -. size 1) in
   let pad32 = Lib.RawIntTypes.size_from_UInt32
     (FStar.Int.Cast.uint8_to_uint32
@@ -183,25 +92,3 @@ let aes256_cbc_decrypt out key iv cip ciplen =
   let msglen = ciplen -. pad32 in
   pop_frame();
   msglen
-
-val aes256_cbc_decrypt_no_pad:
-  out:buffer uint8 ->
-  key:lbuffer uint8 keylen ->
-  iv:block ->
-  cip:buffer uint8{length cip == length out} ->
-  ciplen:size_t{v ciplen = length cip /\ (v ciplen / 16) * 16 + 16 <= max_size_t /\ v ciplen > 0 /\ v ciplen % 16 = 0} ->
-  Stack size_t
-    (requires (fun h -> live h out /\ live h key /\ live h iv /\ live h cip /\
-      disjoint out key /\ disjoint out iv /\ disjoint out cip
-    ))
-    (ensures (fun h0 _ h1 -> modifies1 out h0 h1))
-
-let aes256_cbc_decrypt_no_pad out key iv cip ciplen =
-  push_frame();
-  let kex = create xkeylen (u8 0) in
-  let tmp = create (size 16) (u8 0) in
-  keyExpansion key kex;
-  cbc_decrypt_blocks out kex iv cip ciplen (size 0) tmp;
-  pop_frame();
-  ciplen
-*)
